# Two Body Problem

## Equations of Motion for the Two body problem

Let $\vec{R}_1$ and $\vec{R}_2$ denote the position vectors of masses $m_1$ and $m_2$ in an inertial reference frame. According to Newton‚Äôs Second Law and the law of gravitation:

$$
m_1\ddot{\vec{R}}_1=-G\frac{m_1 m_2}{r^3} \vec{r}
$$ {#eq-f12}

$$
m_2\ddot{\vec{R}}_2=G\frac{m_1 m_2}{r^3} \vec{r}
$$ {#eq-f21}

where $\vec{r}= \vec{R}_2-\vec{R}_1$.

![Diagram of two masses in an inertial frame *OXYZ* (@curtis2005orbital)](fig2_1.jpeg){width="253"}

### Deriving the relative equation of motion

Substituting @eq-f12 and @eq-f21 to $\vec{r}= \vec{R}_2-\vec{R}_1$:

$\ddot{\vec{r}}= -G\frac{m_1 m_2}{r^3}\vec{r}\left(\frac{1}{m_2}+\frac{1}{m_1}\right)= -G \frac{m_1+m_2}{r^3} \vec{r}$

Let the gravitational ùúá parameter be defined as:

$$
\mu= G(m_1+m_2)
$$

Hence the final equation that we use turns out to be:

$$
\boxed{\ddot{\vec{r}}=-\frac{\mu}{r^3}\vec{r}}
$$ {#eq-relmotion}

### Motion of Center of Mass

The center of mass vector is: $\vec{R}_G=\frac{m_1\vec{R}_1+m_2\vec{R}_2}{m_1+m_2}$

Using @eq-f12 and @eq-f21 :

$$
\ddot{\vec{R}}_G= \frac{m_1\ddot{\vec{R}}_1+m_2\ddot{\vec{R}}_2}{m_1+m_2}
$$ {#eq-com}

$$
\ddot{\vec{R}}_G=\frac{-G\frac{m_1m_2}{r^3}\vec{r}+G\frac{m_1m_2}{r^3}\vec{r}}{m_1+m_2}=0
$$

Hence proved that the acceleration of center of mass is zero.

## Angular momentum in two body problem {#sec-angularmom}

The angular momentum of body $m_2$ relative to $m_1$ is moment of $m_2$'s relative linear momentum $m_2 \dot{\vec{r}}$:

$$
\vec{H}_{2/1}= \vec{r} \times m_2\dot{\vec{r}}
$$

where $\dot{\vec{r}}$ is the velocity of $m_2$ relative to $m_1$. We divide this equation of the mass term and get the specific relative angular momentum:

$$
\vec{h}= \vec{r}\times\dot{\vec{r}}
$$

On calculating the time derivative:

$$
\frac{d\vec{h}}{dt}=\dot{\vec{r}}\times\dot{\vec{r}}+ \vec{r}\times \ddot{\vec{r}}
$$

From the @eq-relmotion, we see that $\ddot{\vec{r}} \parallel \vec{r}$ . Hence $\frac{d\vec{h}}{dt}=0 \Rightarrow \vec{h}$ is conserved.

### Eccentricity of orbit from Laplace Runge Lenz vector

Differentiating $\dot {\vec r} \times \vec h$:

$$
\frac{d}{dt}(\dot{\vec r}\times\vec h)= \ddot{\vec r}\times\vec h + \dot{\vec r}\times\underbrace{\dot{\vec h}}_{0}= -\frac{\mu}{r^{3}}\vec r\times(\vec r\times\dot{\vec r})
$$ {#eq-init}

Using the triple product identity $\vec{a}\times(\vec{b}\times\vec{c})=(\vec{a}\cdot\vec{c})\vec b-(\vec a \cdot \vec b)\vec c$ :

$$
\vec r\times(\vec r\times\dot{\vec r})= (\vec r\cdot\dot{\vec r})\vec r - r^{2}\dot{\vec r}
$$

And using the identity $\vec r \cdot \dot{\vec r}=r\dot r$(See [@sec-rrdot] ), we get:

$$ 
\vec r\times(\vec r\times\dot{\vec r})= (r\dot r)\vec r - r^{2}\dot{\vec r} 
$$ {#eq-rcrossrcrossrdot}

Inserting @eq-rcrossrcrossrdot into @eq-init :

$$
\frac{d}{dt}(\dot{\vec r}\times \vec h)=- \frac{\mu}{r^3}\left[(r \dot{r})\vec r - r^2 \dot{\vec r}\right]=-\mu \left[\frac{\dot r \vec r-r\dot{\vec r}}{r^2}\right]
$$ {#eq-six}

But ,

$$
\frac{d}{dt}\left(\frac{\vec r}{r}\right)= \frac{r\dot{\vec r}-\dot r\vec r}{r^2}=-\frac{\dot r\vec r-r\dot{\vec r}}{r^2}
$$

substituting the above into @eq-six;

$$
\frac{d}{dt}\left(\dot{\vec r}\times \vec h\right)= \frac{d}{dt}\left(\mu\frac{\vec r}{r}\right)
$$

Which on integration, gives this solution:

$$
\frac{1}{\mu}(\dot{\vec{r}}\times \vec h)-\frac{\vec r}{r}=\vec e
$$ {#eq-eccvector}

where $\vec e$ is the constant of integration and called as the Laplace-Runge-Lenz Vector. The significance of this vector is that its magnitude $|\vec e|$ gives the eccentricity $e$ and it faces in the direction of the periapsis of the orbit.

## Orbit Equation (Trajectory Under Gravity)

@eq-eccvector is the vector equation that represents the relative motion of one body wrt the other in two body problem. In order to obtain the scalar form, we take a dot product with $\vec r$:

$$
\frac{1}{\mu}(\dot{\vec{r}}\times \vec h)\cdot \vec r-\frac{\vec r\cdot \vec r}{r}=\vec e\cdot \vec r
$$

Using the identity $\vec a \cdot (\vec b \times \vec c)=(\vec a \times \vec b)\cdot \vec c$;

$$
\frac{1}{\mu}\underbrace{(\vec r \times \dot{\vec r})}_{\vec h}\cdot \vec h- \frac{\vec r\cdot\vec r}{r}=\vec e\cdot\vec r
$$

$$
\frac{h^2}{\mu}-r=re\cos{\theta} \text{ where } \theta \text{ is the true anomaly angle }
$$

![The true anomaly $\theta$ is the angle between the eccentricity vector $\vec{e}$ and the position vector $\vec{r}$.](fig2_2.jpeg){width="231"}

Hence the final equation of orbit will turn out to be as follows:

$$
\boxed{r=\frac{\frac{h^2}{\mu}}{1+e\cos{\theta}}}
$$

## Two body problem simulation